wip: added concat proof but correct read proof wip

FormalUrchin/compile.lean
@@ -1,13 +1,13 @@
 import FormalUrchin.units
 import FormalUrchin.mirlight
-import Formal.oseairlight
+import FormalUrchin.oseairlight
 
 import Lean.Data.AssocList
 
 namespace compiler
 
 structure CompileCtx where
-  placemap : Lean.AssocList mir.BasePlace (mir.TyVal × oseair.Register)
+  placemap : Lean.AssocList BasePlace (TyVal × oseair.Register)
   prog : oseair.Prog
   regSuffix : Nat
   currBB: Nat
@@ -27,56 +27,149 @@ inductive CompileExprResult
 | Err (message : String)
 
 
--- def genCopyOpPtr, genLhsPtr
+def insertStmtsInCurrBB (stmts: List oseair.Stmt) (cctx: CompileCtx) : CompileResult :=
+  match cctx.prog.find? cctx.currBB with
+  | none => CompileResult.Err s!"Basic block {cctx.currBB} not found in compile context."
+  | some stmtList =>
+    let newProg := (cctx.prog.erase cctx.currBB).insert cctx.currBB (stmtList ++ stmts)
+    let newCctx := { cctx with prog := newProg }
+    CompileResult.Ok newCctx
 
-def PlaceToReg (v: oseair.Register) (place: mir.Place) (ty: mir.TyVal) (cctx: CompileCtx) : CompileExprResult :=
+-- def genCopyOpPtr, genLhsPtr
+def PlaceToRegWTy (v: oseair.Register) (place: mir.Place) (ty: TyVal) (cctx: CompileCtx) : CompileExprResult :=
   match place with
   | [] => CompileExprResult.Err s!"Empty place"
   | _ => let offset := mir.getPlaceOffset place ty
     match offset with
     | none => CompileExprResult.Err s!"Offset not found for place {place}"
-    | some o =>
-      let (newRegSuffix, newCctx) := freshRegSuffix cctx
-      let newPtr := oseair.Register.P newRegSuffix
-      let stmt := oseair.Stmt.assgn newPtr (oseair.Rhs.bor_offset v o)
-      match newCctx.prog.find? newCctx.currBB with
-      | none => CompileExprResult.Err s!"Basic block {newCctx.currBB} not found in compile context."
-      | some stmtList =>
-        let newProg := newCctx.prog.insert newCctx.currBB (stmtList ++ [stmt])
-        let newCctx1 := { newCctx with prog := newProg }
-        CompileExprResult.Ok newPtr newCctx1
+    | some o => if o == 0 then CompileExprResult.Ok v cctx
+      else
+        let (newRegSuffix, newCctx) := freshRegSuffix cctx
+        let newPtr := oseair.Register.P newRegSuffix
+        let stmt := oseair.Stmt.assgn newPtr (oseair.Rhs.bor_offset v o)
+        match insertStmtsInCurrBB [stmt] newCctx with
+        | CompileResult.Err msg => CompileExprResult.Err msg
+        | CompileResult.Ok newCctx1 => CompileExprResult.Ok newPtr newCctx1
+
+
+
+def PlaceToReg (place: mir.Place) (cctx: CompileCtx) : CompileExprResult :=
+  match place with
+  | [] => CompileExprResult.Err s!"Emply place"
+  | base :: _ => match cctx.placemap.find? base with
+    | none => CompileExprResult.Err s!"Base place {base} not found in compile context."
+    | some (ty, reg) => PlaceToRegWTy reg place ty cctx
+
 
 def compileStmt (stmt: mir.Stmt) (cctx: CompileCtx) : CompileResult :=
   match stmt with
   | mir.Stmt.Assgn lplace rexpr =>
        match rexpr with
-      | mir.RExpr.CopyOp srcPlace =>
-        match cctx.placemap.find? srcPlace with
-        | none => CompileStmtResult.Err s!"Place {srcPlace} not found in context."
-        | some (ty', srcReg) =>
-          if ty == ty' then
-            let stmt := oseair.Stmt.memcpy dstReg srcReg
-            CompileStmtResult.Ok [stmt] cctx
-          else
-            CompileStmtResult.Err s!"Type mismatch: {ty} != {ty'}"
-      | _ => CompileStmtResult.Err "Only CopyOp is supported for now."
-    match lplace with
-    | base :: _ => match cctx.ctx.find? base with
-                    | none =>
-                      let (newRegSuffix, newCctx) := freshRegSuffix cctx
-                      let newPtr := oseair.Register.P newRegSuffix
-                      let allocStmt := oseair.Stmt.assgn newPtr (oseair.Rhs.alloc (mir.TyVal.PtrTy 0))
-    let updatedCtx := newCctx.ctx.insert lplace (ty, newReg)
-    CompileStmtResult.Ok [allocStmt] { newCctx with ctx := updatedCtx }
-    | some (ty, dstReg) =>
+      | mir.RExpr.CopyOp (rbase::rest) =>
+          match cctx.placemap.find? rbase with
+          | none => CompileResult.Err s!"Place {rbase} not found in context."
+          | some (rty, _) =>
+            match PlaceToReg (rbase::rest) cctx with
+            | CompileExprResult.Err msg => CompileResult.Err msg
+            | CompileExprResult.Ok srcReg rhsCCtx =>
+              match lplace with
+              | base :: _ => match cctx.placemap.find? base with
+                              | none =>
+                                let (newRegSuffix, newCctx) := freshRegSuffix rhsCCtx
+                                let dstReg := oseair.Register.P newRegSuffix
+                                let allocStmt := oseair.Stmt.assgn dstReg (oseair.Rhs.alloc rty)
+                                let memcpyStmt := oseair.Stmt.memcpy dstReg srcReg rty -- since rty == lty
+                                insertStmtsInCurrBB [allocStmt, memcpyStmt] newCctx
+                              | some (_ty, dstReg) =>
+                                -- check that _ty == rty
+                                let memcpyStmt := oseair.Stmt.memcpy dstReg srcReg rty -- since rty == lty
+                                insertStmtsInCurrBB [memcpyStmt] rhsCCtx
+              | [] => CompileResult.Err "Empty place"
+      | _ => CompileResult.Err "Only CopyOp is supported for now."
+  | mir.Stmt.Halt => insertStmtsInCurrBB [oseair.Stmt.halt] cctx
 
 
-  match getPlaceAddr place env with
-  | none => none
-  | some addr =>
-    let srcReg := oseair.Register.P addr
-    let dstReg := oseair.Register.P (addr + 1) -- Assuming destination register is next to source
-    let stmt := oseair.Stmt.memcpy dstReg srcReg
-    some (stmt, env, mem, ap)
+  def CompileBB (prog: mir.Prog) (bbNum: Nat) (cctx: CompileCtx) : CompileResult :=
+    match prog.find? bbNum with
+    | none => CompileResult.Err s!"Basic block {bbNum} not found in compile context."
+    | some stmts =>
+      let rec compileStmtsAux (stmts: List mir.Stmt) (cctx: CompileCtx) : CompileResult :=
+        match stmts with
+        | [] => CompileResult.Ok cctx
+        | stmt :: rest =>
+          match compileStmt stmt cctx with
+          | CompileResult.Err msg => CompileResult.Err msg
+          | CompileResult.Ok newCctx =>
+            compileStmtsAux rest newCctx
+      compileStmtsAux stmts cctx
+
+
+  def MirMemoryToOSeairMemory (mem: mir.MemMap) (env: mir.Env) : oseair.MemMap :=
+    let f := fun v ↦
+      match v with
+      | mir.MemValue.Val n => oseair.Val.Dat n
+      | mir.MemValue.Undef => oseair.Val.Undef
+      | mir.MemValue.PlaceTag place tag =>
+        match mir.getPlaceAddr place env with
+        | none => oseair.Val.Undef
+        | some addr => oseair.Val.Ptr addr tag
+    Lean.AssocList.mapVal f mem
+
+-- TODO: Can we break this up into smaller lemmas?
+  theorem mir_conc_step :
+    ∀
+    (N : Word) (bb: BB) (pc: PC) (pc' : PC) (ap: accessperm.AccessPerms) (ap' : accessperm.AccessPerms)
+    (prog: mir.Prog) (mem: mir.Mem) (env: mir.Env)
+    (mem': mir.Mem),
+    -- mir step
+    (prog.find? bb = some [mir.Stmt.Assgn [1] (mir.RExpr.CopyOp [0])]) →
+    (env.find? 0 = some (0, NatTy, 0)) →
+    (mem.mMap.find? 0 = some (mir.MemValue.Val 42)) →
+    mir.Eval2 (bb, pc, prog, env, mem, ap) (bb, pc', prog, env', mem', ap') →
+    -- conclusion
+    mem'.mMap.find? 1 = some (mir.MemValue.Val 42) := by
+      intros N bb pc pc' ap ap'
+            prog mem env
+            mem'
+            h_cpy_stmt h_srcInEnv h_valInMem h_mirstep
+      cases h_mirstep
+      case AssgnRel h1 h2_lplace h3_rplace h4 h5 h6 h7 h8 h9 h10 =>
+        have : h2_lplace = [1] := by
+          rw [h8] at h_cpy_stmt
+          
+
+  -- TODO: Can we break this up into smaller lemmas?
+  theorem bisim_copy :
+    ∀
+    (N : Word) (bb: BB) (pc: PC) (pc' : PC) (ap: accessperm.AccessPerms) (ap' : accessperm.AccessPerms)
+    (prog: mir.Prog) (cctx: CompileCtx) (mem: mir.Mem) (env: mir.Env)
+    (srcplace: mir.Place) (srcaddr: Addr) (srcty: TyVal) (srctag: Tag) (destplace: mir.Place)
+    (mem': mir.Mem)
+    (seaRegMap : oseair.RegMap) (seaRegMap': oseair.RegMap)
+    (seaMem: oseair.Mem) (seaMem': oseair.Mem),
+    -- mir step
+    (prog.find? bb = some [mir.Stmt.Assgn destplace (mir.RExpr.CopyOp (srcbase :: srcrest))]) →
+    (env.find? srcbase = some (srcaddr, srcty, srctag)) →
+    (mem.mMap.find? srcaddr = some (mir.MemValue.Val N)) →
+    mir.Eval2 (bb, pc, prog, env, mem, ap) (bb, pc', prog, env', mem', ap') →
+    -- compiler function
+    compileStmt stmt cctx = CompileResult.Ok cctx' →
+    (cctx.placemap.find? srcbase = some (srcty, oseair.Register.P 0)) →
+    -- oseair step
+    oseair.Eval (seaBB, seaPC, cctx'.prog, seaReg, seaMem, seaAP) (seaBB, seaPC', cctx'.prog, seaReg', seaMem', seaAP')  →
+    MirMemoryToOSeairMemory mem.mMap env = seaMem.mMap →
+    -- conclusion
+    MirMemoryToOSeairMemory mem'.mMap env' = seaMem.mMap := by
+    intros N bb pc pc' ap ap'
+          prog cctx mem env srcplace
+          srcaddr srcty srctag destplace mem'
+          seaRegMap seaRegMap' seaMem seaMem'
+          h_cpy_stmt h_srcInEnv h_valInMem h_mirstep
+          h_compile_ok h_srcRegInPlacemap h_oseairstep
+          h_init_mem_eq
+    cases h_mirstep
+    sorry
+
+-- assumption:  The BB can be traversed in an order that respects topological sort
 
 end compiler
