FormalUrchin/units.lean
@@ -1,5 +1,38 @@
+-- This file contains the definitions of the types used in the formalization of the Urchin language.
+import Lean.Data.AssocList
+
 abbrev Word := Nat
 abbrev BasePlace := Word
 abbrev BasicBlock := Word
 abbrev Place := List Word
 abbrev Tag := Word
+abbrev BB := Word
+abbrev PC := Word
+abbrev AddrStart := Word
+abbrev Addr := Word
+
+inductive TyVal
+| NatTy : TyVal
+| PTy : TyVal
+| TupTy : List TyVal → TyVal
+
+partial def TyVal.toString : TyVal → String
+  | TyVal.NatTy => s!"NatTy"
+  | TyVal.PTy => s!"PlaceTy"
+  | TyVal.TupTy tys  =>
+    let _ : ToString TyVal := ⟨TyVal.toString⟩
+    s!"TupTy({String.intercalate ", " (tys.map toString)})"
+
+instance : ToString TyVal where
+  toString := TyVal.toString
+
+partial def TyVal.beq : TyVal → TyVal → Bool
+  | TyVal.NatTy, TyVal.NatTy => true
+  | TyVal.PTy , TyVal.PTy => true
+  | .TupTy (ty1 :: rest1), .TupTy (ty2::rest2) =>
+    let _ : BEq TyVal := ⟨TyVal.beq⟩
+    ty1 == ty2 && rest1 == rest2
+  | _, _ => false
+
+instance : BEq TyVal where
+  beq := TyVal.beq
